Logic/Vorspiel/Order.lean
@@ -1,5 +1,7 @@
 import Logic.Vorspiel.Vorspiel
 
+section
+
 variable {α : Sort u} (r : α → α → Prop)
 
 local infix:50 " ≺ " => r
@@ -25,3 +27,29 @@ lemma isInfiniteDescendingChain_of_non_acc (z : α) (hz : ¬Acc r z) :
       exact Classical.epsilon_spec this
   intro i; simpa using (this (i + 1)).1
 
+end
+
+section HeytingAlgebra
+
+variable {α : Type*} [HeytingAlgebra α]
+
+lemma himp_himp_inf_himp_inf_le (a b c : α) : (a ⇨ b ⇨ c) ⊓ (a ⇨ b) ⊓ a ≤ c := calc
+  (a ⇨ b ⇨ c) ⊓ (a ⇨ b) ⊓ a = (a ⇨ b ⇨ c) ⊓ b ⊓ a := by simp only [inf_assoc, himp_inf_self]
+  _                         = (a ⇨ b ⇨ c) ⊓ a ⊓ b := by simp only [inf_assoc, inf_comm a b]
+  _                         ≤ (b ⇨ c) ⊓ b         := by simp only [himp_inf_self a (b ⇨ c), le_inf_iff]
+                                                        constructor
+                                                        · simp only [inf_assoc, inf_le_left]
+                                                        · exact inf_le_right
+  _                         ≤ c                   := by simp
+
+lemma himp_inf_himp_inf_sup_le (a b c : α) : (a ⇨ c) ⊓ (b ⇨ c) ⊓ (a ⊔ b) ≤ c := by
+  have ha : a ≤ (a ⇨ c) ⊓ (b ⇨ c) ⇨ c := by
+    simp only [le_himp_iff, ← inf_assoc, inf_himp]
+    refine inf_le_of_left_le (by simp)
+  have hb : b ≤ (a ⇨ c) ⊓ (b ⇨ c) ⇨ c := by
+    simp only [le_himp_iff, inf_comm (a ⇨ c) (b ⇨ c), ← inf_assoc, inf_himp]
+    refine inf_le_of_left_le (by simp)
+  have : a ⊔ b ≤ (a ⇨ c) ⊓ (b ⇨ c) ⇨ c := sup_le_iff.mpr ⟨ha, hb⟩
+  simpa only [GeneralizedHeytingAlgebra.le_himp_iff, inf_comm (a ⊔ b)] using this
+
+end HeytingAlgebra
